theories/laws/utp_pred_laws.thy
@@ -133,7 +133,7 @@ lemma ImpliesP_export:
   by (utp_pred_tac)
 
 lemma ImpliesP_eq_subst:
-  "v \<rhd>\<^sub>e x \<Longrightarrow> `$x = v \<Rightarrow> p` = `$x = v \<Rightarrow> p[v/x]`"
+  "v \<rhd>\<^sub>e x \<Longrightarrow> (VarE x ==p v) \<Rightarrow>p p = (VarE x ==p v) \<Rightarrow>p p[v|x]"
   apply (utp_pred_tac, utp_expr_tac)
   apply (auto simp add:evale eval typing)
   apply (metis binding_upd_simps(2))+
